Given the points $(x_{1},y_{1}),(x_{2},y_{2}),(x_{3},y_{3})$ The perpendicular bisectors $(h,k)$ will intersect at the circumcentre
$$(h_1, k_1) = \left(\frac{x_1 + x_2}{2}, \frac{y_1 + y_2}{2}\right)$$
$$ (h_2, k_2) = \left(\frac{x_2 + x_3}{2}, \frac{y_2 + y_3}{2}\right)$$
$$ m_{\text{perp1}} = -\frac{1}{\frac{y_2 - y_1}{x_2 - x_1}} $$
$$ m_{\text{perp2}} = -\frac{1}{\frac{y_3 - y_2}{x_3 - x_2}}$$
Equation 1
$$y-k_{1}=m_{perp1}(x-h_{1})$$
$$y=m_{perp1}(x-h_{1})+k_{1}$$
Equation 2
$$y-k_{2}=m_{perp2}(x-h_{2})$$
$$y=m_{perp2}(x-h_{2})+k_{2}$$
AA
$$m_{perp1}(x-h_{1})+k_{1}=m_{perp2}(x-h_{2})+k_{2}$$
$$xm_{perp1}-h_{1}m_{perp1}+k_{1}=xm_{perp2}-h_{2}m_{perp2}+k_{2}$$
$$x(m_{perp1}-m_{perp2})=h_1m_{perp1}-h_{2}m_{perp2}+k_{2}-k_{1}$$
$$x = \frac{h_1m_{perp1}-h_{2}m_{perp2}+k_{2}-k_{1}}{m_{perp1}-m_{perp2}}$$
Plug back into equation
$$y=m_{perp2}(x-h_{2})+k_{2}$$