- Sum of an [[Arithmetic Sequence]]
# Formula
$$S_{n}= \frac{n}{2}(2a + (n-1)d)$$
$$S_{n}= \frac{n}{2}(a + l)$$

| Symbol | Definition |
| ---- | ---- |
| $S_n$ | The series |
| $n$ | size of the series |
| $a$ | first term in the series |
| $d$ | common difference |
| $l$ | last term in the series |
 # Proof Need to know
$$S_{n}= a + (a + d) + (a + 2d) + ...+(a+(n-2)d)+(a+(n-1)d)$$
$$S_{n}=(a+(n-1)d) +(a+(n-2)d) +...+ (a + 2d) +(a + d) + a $$
Add together the two lines
$$2S_{n}=(2a+(n-1)d) + (2a+(n-1)d)+...+(2a+(n-1)d)+(2a+(n-1)d)$$
We have n amount of terms
$$2S_{n}= n(2a + (n-1)d)$$
$$S_{n}= \frac{n}{2}(2a + (n-1)d) $$
# Proof for variation
Last term $l$ in a sequence is
$$l =a + (n-1)d$$
Plug it into equation to get
$$S_{n}= \frac{n}{2}(a + l)$$
