Start at
$ax^2+bx+c=0$
$a(x^2+\frac{b}{a}+\frac{c}{a})=0$
$let \; u = x^2+\frac{b}{a}+\frac{c}{a}$
$then \; au = 0$
$u = (x+\frac{b}{2a})^2 - (\frac{b}{2a})^2 +\frac{c}{a}$
$u = (x+\frac{b}{2a})^2 - \frac{b^2}{4a^2} +\frac{4ac}{4a^2}$
$u = (x+\frac{b}{2a})^2 + \frac{-b^2-4ac}{4a^2}$
plug that $\uparrow$ back into $au=0$
$a((x+\frac{b}{2a})^2 + \frac{-b^2-4ac}{4a^2}) = 0$
$a(x+\frac{b}{2a})^2 + \frac{-b^2-4ac}{4a} = 0$
look at $\circledast$ for turning point
$-\frac{-b^2-4ac}{4a}$
$a(x+\frac{b}{2a})^2 = -\frac{-b^2-4ac}{4a}$
$\div a$
$(x+\frac{b}{2a})^2 = -\frac{-b^2-4ac}{4a^2}$
$\sqrt{ }$
$x+\frac{b}{2a} = -\frac{\sqrt{-b^2-4ac}}{2a}$
$-\frac{b}{2a}$
$x = \frac{-b\pm \sqrt{b^2-4ac}}{2a}$

$\circledast$
$y=a(x+\frac{b}{2a})^2 + \frac{-b^2-4ac}{4a}$
when $x=-\frac{b}{2a},y=\frac{-b^2-4ac}{4a}$ and graph is at a minimum
so minimum at $(-\frac{b}{2a},\frac{-b^2-4ac}{4a})$