Sum of all terms in a [[Geometric Sequence]]
# Formula for finite
$$S_n=\frac{a(1-r^{n})}{1-r}$$
## Proof (Need to know)
Let
$$s_{n}= a + ar + ar^{2}+ ar^{3}+..+ar^{n-2} + ar^{n-1}$$
$$rS_{n} = ar + ar^{2}+ ar^{3}+..+ar^{n-1} + ar^{n}$$
$$S_{n}-rS_{n}= a-ar^n$$
$$S_{n}(1-r)= a(1-r^{n})$$
$$S_{n} = \frac{a(1-r^n)}{1-r}$$
# Formula for infinite
$$S_{\infty}= \frac{a}{1-r} \ \ \ \ \text{if  } |r| < 1$$
## Proof (Need to know)
if $-1 < r < 1$ then as $n \rightarrow \infty, \ r^{n} \rightarrow 0$
So
$$S_{\infty}= \frac{a(1-0)}{1-r}$$
$$S_{\infty}= \frac{a}{1-r} \ \ \ \ \text{if  } |r| < 1$$