- $𝑦 = 𝑎𝑓(𝑥)$ 
would stretch the graph in the vertical direction by a multiple of 𝑎
$(x,y)$ becomes $(x,ay)$

- $y=f(ax)$
would stretch the graph in the horizontal direction by a multiple of $\frac{1}{a}$
$(x,y)$ becomes $(\frac{x}{a},y)$

- $y=-f(x)$
reflection of $f(x)$ in the x-axis
$(x,y)$ becomes $(x,-y)$

- $y=f(-x)$
reflection of $f(x)$ in the y-axis
$(x,y)$ becomes $(-x,y)$

- $y=f(x)+a$
moves graph in y axis by factor of a
$(x,y)$ becomes $(x,y+a)$

- $y=f(x+a)$
moves graph in x axis by factor of -a
$(x,y)$ becomes $(x-a,y)$
